Modified REDUCE_ss (used in std_ss, and in a lot of other places too) to reduce terms of the form SUC (SUC (SUC ... n)..)) where n is a numeral. This breaks a few proofs, but not a huge number.  It seems silly to have REDUCE_CONV do one thing (reduce ground SUC terms) but not REDUCE_ss.

src/num/arith/src/numSimps.sml
@@ -367,6 +367,7 @@ val REDUCE_ss = simpLib.SIMPSET
   {convs = mk_unary_rconv (--`EVEN`--) ::
            mk_unary_rconv (--`ODD`--)  ::
            mk_unary_rconv (--`PRE`--)  ::
+           mk_unary_rconv (--`SUC`--) ::
            map mk_redconv [--`$*`--, --`$+`--, --`$-`--,
                            --`$DIV`--, --`$MOD`--, --`$EXP`--,
                            --`$<`--, --`$<=`--, --`$>`--,
